src/test_sem.v
@@ -6,7 +6,7 @@ Goal
     forall arch prog type_ctxt ctxt opt_ctxt' var typ dir,
         find_val type_ctxt var = Some typ ->
         well_typed_ctxt type_ctxt ctxt ->
-        convert_type typ nil = Some (dir, 1::nil) ->
+        convert_type typ = Some (dir, 1::nil) ->
         find_val ctxt var = None ->
         eval_deq arch prog type_ctxt ctxt
             (Eqn (Index (Var var) (Const_e 0%Z) :: (Index (Var var) (Const_e 0%Z)) :: nil) (Tuple (ECons (Const 1 None)
@@ -33,13 +33,13 @@ Goal
     forall arch prog type_ctxt ctxt opt_ctxt' var typ dir,
         find_val type_ctxt var = Some typ ->
         well_typed_ctxt type_ctxt ctxt ->
-        convert_type typ nil = Some (dir, 1::nil) ->
+        convert_type typ = Some (dir, 1::nil) ->
         (exists v, eval_var (Index (Var var) (Const_e 0)) ctxt AAll = Some v) ->
         eval_deq arch prog type_ctxt ctxt
             (Eqn (Index (Var var) (Const_e 0%Z) :: (Index (Var var) (Const_e 0%Z)) :: nil) (Tuple (ECons (Const 1 None)
                             (ECons (Const 2 None) Enil)))
                 true) = opt_ctxt'
-        -> (ctxt' <- opt_ctxt'; find_val ctxt' var) = Some (CoIR dir (Some 2%Z::nil) (Some (1::nil))).
+        -> (ctxt' <- opt_ctxt'; find_val ctxt' var) = Some (CoIR dir (Some 2%Z::nil) (1::nil)).
 Proof.
     simpl.
     unfold bind; unfold bind_aux_list.
@@ -69,8 +69,6 @@ Proof.
             rewrite PeanoNat.Nat.mul_1_l in Abs; discriminate.
         }
         destruct valoType as [FormEq length_eq].
-        destruct form as [form|].
-        2: by destruct FormEq.
         symmetry in FormEq; destruct FormEq; simpl.
         simpl in length_eq.
         rewrite mul1n in length_eq.
@@ -98,13 +96,13 @@ Goal
     forall arch prog type_ctxt ctxt opt_ctxt' var typ dir,
         find_val type_ctxt var = Some typ ->
         well_typed_ctxt type_ctxt ctxt ->
-        convert_type typ nil = Some (dir, 2::nil) ->
+        convert_type typ = Some (dir, 2::nil) ->
         find_val ctxt var = None ->
         eval_deq arch prog type_ctxt ctxt
              (Eqn (Range (Var var) (Const_e 1) (Const_e 0)::nil) (Tuple (ECons (Const 1 None)
                             (ECons (Const 2 None) Enil)))
                 false) = opt_ctxt'
-        -> (ctxt' <- opt_ctxt'; find_val ctxt' var) = Some (CoIR dir (Some 2::Some 1::nil)%Z (Some (2::nil))).
+        -> (ctxt' <- opt_ctxt'; find_val ctxt' var) = Some (CoIR dir (Some 2::Some 1::nil)%Z (2::nil)).
 Proof.
     simpl.
     unfold bind; unfold bind_aux_list.
@@ -124,18 +122,44 @@ Proof.
     }
 Qed.
 
+Require Import Lia.
+
+Lemma divmod_change_rem:
+    forall n p u q1 q2, (Nat.divmod n p q1 u).2 = (Nat.divmod n p q2 u).2.
+Proof.
+    move=> n; induction n as [|n HRec]; simpl; trivial.
+    move=> p [|u] q1 q2; apply HRec.
+Qed.
+
+Lemma eq_divmod:
+    forall n u q, (u < 2)%coq_nat -> (Nat.divmod n 1 q u).2 = (u + n) mod 2.
+Proof.
+    move=> n; induction n as [|n HRec]; simpl; trivial.
+    {
+        move=> u _; destruct u as [|[]]; simpl; auto.
+        lia.
+    }
+    destruct (Nat.mod_bound_pos n 2); auto.
+    by lia.
+    move=> [|u] q Bound; rewrite HRec; trivial.
+    1,3: lia.
+    simpl.
+    unfold addn_rec; rewrite Nat.add_succ_r; simpl.
+    rewrite (divmod_change_rem _ _ _ 0 1); reflexivity.
+Qed.
+
 Goal
     forall arch prog type_ctxt ctxt opt_ctxt' var typ dir,
         find_val type_ctxt var = Some typ ->
         well_typed_ctxt type_ctxt ctxt ->
-        convert_type typ nil = Some (dir, 2::nil) ->
+        convert_type typ = Some (dir, 2::nil) ->
         (exists v, eval_var (Index (Var var) (Const_e 0)) ctxt AAll = Some v) ->
         (exists v, eval_var (Index (Var var) (Const_e 1)) ctxt AAll = Some v) ->
         eval_deq arch prog type_ctxt ctxt
              (Eqn (Range (Var var) (Const_e 1) (Const_e 0)::nil) (Tuple (ECons (Const 1 None)
                             (ECons (Const 2 None) Enil)))
                 true) = opt_ctxt'
-        -> (ctxt' <- opt_ctxt'; find_val ctxt' var) = Some (CoIR dir (Some 2::Some 1::nil)%Z (Some (2::nil))).
+        -> (ctxt' <- opt_ctxt'; find_val ctxt' var) = Some (CoIR dir (Some 2::Some 1::nil)%Z (2::nil)).
 Proof.
     simpl.
     unfold bind; unfold bind_aux_list.
@@ -150,64 +174,75 @@ Proof.
         destruct p as [typ' [find_typ valoType]].
         rewrite find_typ in HEqType; inversion HEqType as [HEq'].
         destruct HEq'; clear HEqType.
-        destruct typ' as [|d m n|typ len]; simpl in Convert.
+        destruct typ' as [|d m n|typ ilen]; simpl in *.
         by discriminate.
         all: swap 1 2.
         {
-            destruct (eval_arith_expr nil len) as [ilen|].
-            2: by discriminate.
+            destruct typ as [|d m n|typ len2]; simpl in *.
+            by discriminate.
+            {
+                destruct m; destruct n; destruct d; inversion Convert as [[Hdir Hilen]].
+                all: destruct Hdir; symmetry in Hilen; destruct Hilen.
+                all: destruct c.
+                1,3,5,7,9-14: destruct valoType.
+                all: destruct valoType as [H [NotEmpty [LengthEq DirEq]]]; symmetry in H; destruct H.
+                4: by destruct DirEq.
+                all: symmetry in LengthEq; destruct LengthEq; symmetry in DirEq; destruct DirEq.
+                all: rewrite muln1; simpl.
+                all: destruct l as [|h1 [|h2 []]].
+                1,2,4-6,8-10,12: move=> H; destruct H as [v Abs]; inversion Abs.
+                all: simpl; destruct h1 as [h1|].
+                2,4,6: move=> H; destruct H as [v Abs]; inversion Abs.
+                all: simpl; destruct h2 as [h2|].
+                2,4,6: move=> _ H; destruct H as [v Abs]; inversion Abs.
+                all: simpl; move=> _ _ <-; simpl; rewrite ident_beq_refl; reflexivity.
+            }
             exfalso; move: Convert.
-            clear.
-            pose (p := [:: ilen]); fold p.
-            assert (p <> nil) as NotEmpty by (unfold p; move=> Eq; discriminate).
+            pose (p := [:: len2; ilen]); fold p.
+            assert (length p > 1) as NotEmpty
+             by (unfold p; simpl; constructor).
             move: p NotEmpty; clear.
             induction typ as [|d m n|typ HRec len']; simpl.
             by discriminate.
             {
                 destruct m.
-                + move=> []; destruct d; auto.
-                    4,6: by discriminate.
-                    1-3: by move=> a []; simpl; discriminate.
-                    by move=> a []; discriminate.
+                + move=> []; destruct n; destruct d; auto.
+                    1-12: move=> a l HDiff HEq; inversion HEq as [[H H1 H2]].
                 + discriminate.
-                + move=> [|hd tl] HNeq.
-                    - exfalso; apply HNeq; reflexivity.
-                    - destruct d; destruct tl; discriminate.
+                + move=> []; destruct n; destruct d; auto.
+                    1-12: move=> a l HDiff HEq; inversion HEq as [[H H1 H2]].
             }
             {
-                destruct (eval_arith_expr nil len').
-                2: by discriminate.
-                move=> [|hd tl] NotEmpty.
-                by exfalso; apply NotEmpty; reflexivity.
-                apply HRec.
-                discriminate.
+                move=> p NotEmpty.
+                destruct convert_type as [[d l]|]; by idtac.
             }
         }
         simpl in *.
         destruct m as [| |].
         2,3: by destruct valoType.
         destruct c as [|d' l form]; simpl.
-        {
-            by destruct valoType.
-        }
+        by move=> [v H]; inversion H.
         destruct form.
+        by move=> [v H]; inversion H.
+        destruct n as [n|].
         2: by destruct valoType.
         rewrite muln1 in valoType.
+        destruct valoType as [H1 [NotEmpty [length_eq dir_eq]]].
+        move: HEq.
+        inversion H1; clear H0 H2 H1 n1 form.
+        move=> HEq.
         destruct d.
-        4: by discriminate.
-        5: by discriminate.
+        4,6: by discriminate.
         all: inversion Convert as [[HEq2 HEq3]]; clear Convert; simpl.
         all: destruct HEq2.
         all: symmetry in HEq3; destruct HEq3.
-        all: destruct valoType as [simpl_eq [_ [length_eq dir_eq]]].
-        all: rewrite length_eq; simpl.
         all: destruct l as [|h1 l].
         1,3,5,7: by discriminate.
         all: destruct l as [|h2 l].
         1,3,5,7: by discriminate.
         all: destruct l as [|].
         2,4,6,8: by discriminate.
-        all: rewrite simpl_eq; simpl.
+        all: simpl.
         all: destruct h1.
         2,4,6,8: by move=> []; discriminate.
         all: destruct h2.
