src/testing/aes.v
@@ -1,0 +1,116 @@
+(*
+Here b8[16] = b1[16][8] is represented as T16 (T8 Atom)
+*)
+
+Section Test.
+Variables (Prod : Type -> Type -> Type).
+
+Class Array (T : Type -> Type) := {
+    MAP : forall A B, (A -> B) -> T A -> T B;
+    pure : forall A, A -> T A;
+    functor : forall A B, T (A -> B) -> T A -> T B;
+    pair : forall A B, T A -> T B -> T (Prod A B)
+}.
+
+Class Indexable (T : Type -> Type) := {
+    array : Array T;
+    IndType : Type;
+    lookup : (forall A, T A -> IndType -> A);
+}.
+
+Class Logic (A : Type) := {
+    Not : A -> A;
+    Xor : A -> A -> A;
+    Or  : A -> A -> A;
+    And : A -> A -> A;
+    Andn: A -> A -> A;
+}.
+
+Variables (Atom : Type) (LAtom : Logic Atom).
+Variables (T4 : Type -> Type) (IT4 : Indexable T4).
+Variables (Build4 : forall A, A * A * A * A -> T4 A).
+Variables (I4a I4b I4c I4d : @IndType T4 _).
+Variables (T8 : Type -> Type) (AT8 : Array T8).
+Variables (T11 : Type -> Type) (IT11 : Indexable T11).
+Variables (I11a I11b I11c I11d I11e I11f I11g I11h I11i I11j I11k : @IndType T11 _).
+Variables (T16 : Type -> Type) (IT16 : Indexable T16).
+Variables (T32 : Type -> Type).
+Variables (T128 : Type -> Type) (AT128 : Array T128).
+
+Variables
+    (T32_split : forall A, T32 A -> T4 (T8 A))
+    (T32_merge : forall A, T4 (T8 A) -> T32 A).
+Variables
+    (T128_split : forall A, T128 A -> T16 (T8 A))
+    (T128_merge : forall A, T16 (T8 A) -> T128 A)
+    (T128_split' : forall A, T128 A -> T4 (T32 A))
+    (T128_merge' : forall A, T4 (T32 A) -> T128 A).
+
+Variables (SubBytes_singles : forall A, T8 A -> T8 A).
+
+Definition SubBytes : T16 (T8 Atom) -> T16 (T8 Atom) :=
+    @MAP _ array _ _ (SubBytes_singles _).
+
+Variables (Indexes : T16 (@IndType T16 _)).
+
+Definition ShiftRows : T16 (T8 Atom) -> T16 (T8 Atom) :=
+    fun el => @MAP _ array _ _ (lookup _ el) Indexes.
+
+Variables (VectorTimes2 : T8 Atom -> T8 Atom).
+
+Variables (ShiftL : nat -> T8 Atom -> T8 Atom).
+
+Definition times2 : T8 Atom -> T8 Atom :=
+    fun l => functor _ _ (MAP _ _ Xor (ShiftL 1 l)) (VectorTimes2 l).
+
+Definition times3 : T8 Atom -> T8 Atom :=
+    fun i => functor _ _ (MAP _ _ Xor (times2 i)) i.
+
+Definition MixColumn_single : T4 (T8 Atom) -> T4 (T8 Atom) :=
+    fun inp => Build4 _ (
+        functor _ _ (MAP _ _ Xor
+            (functor _ _ (MAP _ _ Xor (times2 (lookup _ inp I4a))) (times3 (lookup _ inp I4b))))
+            (functor _ _ (MAP _ _ Xor (lookup _ inp I4c)) (lookup _ inp I4d))
+        ,
+        functor _ _ (MAP _ _ Xor
+            (functor _ _ (MAP _ _ Xor (lookup _ inp I4a)) (times2 (lookup _ inp I4b))))
+            (functor _ _ (MAP _ _ Xor (times3 (lookup _ inp I4c))) (lookup _ inp I4d))
+        ,
+        functor _ _ (MAP _ _ Xor
+            (functor _ _ (MAP _ _ Xor (lookup _ inp I4a)) (lookup _ inp I4b)))
+            (functor _ _ (MAP _ _ Xor (times2 (lookup _ inp I4c))) (times3 (lookup _ inp I4d)))
+        ,
+        functor _ _ (MAP _ _ Xor
+            (functor _ _ (MAP _ _ Xor (times3 (lookup _ inp I4a))) (lookup _ inp I4b)))
+            (functor _ _ (MAP _ _ Xor (lookup _ inp I4c)) (times2 (lookup _ inp I4d)))
+    ).
+
+Definition MixColumn : T4 (T32 Atom) -> T4 (T32 Atom) :=
+    fun inp =>
+        Build4 _ (
+            T32_merge _ (MixColumn_single (T32_split _ (lookup _ inp I4a))),
+            T32_merge _ (MixColumn_single (T32_split _ (lookup _ inp I4b))),
+            T32_merge _ (MixColumn_single (T32_split _ (lookup _ inp I4c))),
+            T32_merge _ (MixColumn_single (T32_split _ (lookup _ inp I4d)))
+        ).
+
+Definition AddRoundKey : T128 Atom -> T128 Atom -> T128 Atom :=
+    fun i key => functor _ _ (MAP _ _ Xor i) key.
+
+Definition AES : T128 Atom -> T11 (T128 Atom) -> T128 Atom :=
+    fun plain key =>
+        let tmp0 := AddRoundKey plain (lookup _ key I11a) in
+        let tmp1 := AddRoundKey (T128_merge' _ (MixColumn (T128_split' _ (T128_merge _ (ShiftRows (SubBytes (T128_split _ tmp0))))))) (lookup _ key I11b) in
+        let tmp2 := AddRoundKey (T128_merge' _ (MixColumn (T128_split' _ (T128_merge _ (ShiftRows (SubBytes (T128_split _ tmp1))))))) (lookup _ key I11c) in
+        let tmp3 := AddRoundKey (T128_merge' _ (MixColumn (T128_split' _ (T128_merge _ (ShiftRows (SubBytes (T128_split _ tmp2))))))) (lookup _ key I11d) in
+        let tmp4 := AddRoundKey (T128_merge' _ (MixColumn (T128_split' _ (T128_merge _ (ShiftRows (SubBytes (T128_split _ tmp3))))))) (lookup _ key I11e) in
+        let tmp5 := AddRoundKey (T128_merge' _ (MixColumn (T128_split' _ (T128_merge _ (ShiftRows (SubBytes (T128_split _ tmp4))))))) (lookup _ key I11f) in
+        let tmp6 := AddRoundKey (T128_merge' _ (MixColumn (T128_split' _ (T128_merge _ (ShiftRows (SubBytes (T128_split _ tmp5))))))) (lookup _ key I11g) in
+        let tmp7 := AddRoundKey (T128_merge' _ (MixColumn (T128_split' _ (T128_merge _ (ShiftRows (SubBytes (T128_split _ tmp6))))))) (lookup _ key I11h) in
+        let tmp8 := AddRoundKey (T128_merge' _ (MixColumn (T128_split' _ (T128_merge _ (ShiftRows (SubBytes (T128_split _ tmp7))))))) (lookup _ key I11i) in
+        let tmp9 := AddRoundKey (T128_merge' _ (MixColumn (T128_split' _ (T128_merge _ (ShiftRows (SubBytes (T128_split _ tmp8))))))) (lookup _ key I11j) in
+        AddRoundKey (T128_merge _ (ShiftRows (SubBytes (T128_split _ tmp9)))) (lookup _ key I11k)
+    .
+
+
+End Test.
